TransferFunction.v
@@ -1,3 +1,4 @@
+From Coq Require Import ssreflect ssrfun ssrbool.
 Require Export PolyAI.Presburger.
 Require Export PolyAI.AbstractDomain.
 Require Import PolyAI.SSA.
@@ -18,8 +19,132 @@ Class transfer_function {ab: Type} (A: adom ab) :=
                            Ensembles.In RegisterMap (gamma a') R'
   }.
 
-Definition transfer_presburger_set_const {S: Type} {P: PresburgerSet S} (s: S) (l: label) (var: string) (val: nat) :=
-  true.
+Definition transfer_presburger_set_const {S: Type} {P: PresburgerSet S} (s: S) (l: label) (v: string) (c: Z) :=
+  let constraint := CEq (AVar v) (AConst c) in
+  let s := set_project_out s v in
+  let c_set := set_from_constraint constraint in
+  let new_set := intersect_set c_set s in
+  (new_set, l+1).
+
+Lemma transfer_presburger_set_const_sound_aux {S: Type} (P: PresburgerSet S) :
+  forall v c R l R' l', (R', l') = ssa_step (Const v c) R l ->
+                   forall a, Ensembles.In RegisterMap (@gamma S (PresburgerSetAD P) a) R ->
+                        let (a', l') := (transfer_presburger_set_const a l v c) in
+                              Ensembles.In RegisterMap (gamma a') R'.
+Proof.
+  move=> v c R l R' l' [HR' Hl'] a Hingamma.
+  rewrite /Ensembles.In /transfer_presburger_set_const /gamma /= in Hingamma *.
+  rewrite intersect_set_spec Bool.andb_true_iff.
+  split.
+    - by rewrite set_from_constraint_spec /= HR' t_update_eq Z.eqb_refl //.
+    - rewrite set_project_out_spec.
+      exists (R v).
+      rewrite HR' t_update_shadow t_update_same.
+        by exact Hingamma.
+Qed.
+
+Theorem transfer_presburger_set_const_sound {S: Type} (P: PresburgerSet S) :
+  forall v c prog R l R' l',
+    step prog (R, l) (R', l') ->
+    Some (Const v c) = List.nth_error prog l ->
+    forall a, Ensembles.In RegisterMap (gamma a) R ->
+         exists a', In (a', l') ((transfer_presburger_set_const a l v c)::nil) /\
+               Ensembles.In RegisterMap (gamma a') R'.
+Proof.
+  move => v c prog R l R' l' Hstep Hinst a HIn.
+  exists (fst (transfer_presburger_set_const a l v c)).
+  inversion Hstep. subst.
+  rewrite -Hinst in H6.
+  case: H6 => H6.
+  rewrite H6 /= in H7.
+  split.
+  - left.
+    move: H7 => [HR' Hl'].
+    rewrite Hl'.
+    by reflexivity.
+  - move: (transfer_presburger_set_const_sound_aux P v c R l R' l' H7 a HIn) => Hgoal.
+    by apply Hgoal.
+Qed.
+
+Definition binop_to_pwaff (v: variable) (opc: BinArithOpCode) (op1 op2: variable) :=
+  match opc with
+  | OpAdd => APlus (AVar op1) (AVar op2)
+  | OpMul => AVar v
+  | OpLe => ALe (AVar op1) (AVar op2)
+  end.
+
+Definition transfer_presburger_set_binop {S: Type} {P: PresburgerSet S} (s: S) (l: label) (v: variable) (opc: BinArithOpCode) (op1 op2: variable) :=
+  let pwaff := binop_to_pwaff v opc op1 op2 in
+  let constraint := CEq (AVar v) pwaff in
+  let s := set_project_out s v in
+  let c_set := set_from_constraint constraint in
+  let new_set := intersect_set c_set s in
+  (new_set, l+1).
+
+
+Lemma transfer_presburger_set_binop_sound_aux {S: Type} (P: PresburgerSet S) :
+  forall v opc op1 op2 Hop1 Hop2 R l R' l',
+    (R', l') = ssa_step (BinOp v opc op1 op2 Hop1 Hop2) R l ->
+    forall a, Ensembles.In RegisterMap (@gamma S (PresburgerSetAD P) a) R ->
+         let (a', l') := (transfer_presburger_set_binop a l v opc op1 op2) in
+         Ensembles.In RegisterMap (gamma a') R'.
+Proof.
+  move=> v opc op1 op2 Hop1 Hop2 R l R' l' [HR' Hl'] a Hingamma.
+  rewrite /Ensembles.In /transfer_presburger_set_const /gamma /= in Hingamma *.
+  rewrite intersect_set_spec Bool.andb_true_iff.
+  split.
+  - rewrite set_from_constraint_spec /= HR' t_update_eq.
+    case opc;
+      try ((repeat (rewrite /= t_update_neq => [// |]);
+            rewrite Z.eqb_refl //)).
+    + rewrite /= t_update_eq Z.eqb_refl //.
+  - rewrite set_project_out_spec.
+    exists (R v).
+    rewrite HR' t_update_shadow t_update_same.
+      by exact Hingamma.
+Qed.
+
+Theorem transfer_presburger_set_binop_sound {S: Type} (P: PresburgerSet S) :
+  forall v opc op1 op2 Hop1 Hop2 prog R l R' l',
+    step prog (R, l) (R', l') ->
+    Some (BinOp v opc op1 op2 Hop1 Hop2) = List.nth_error prog l ->
+    forall a, Ensembles.In RegisterMap (gamma a) R ->
+         exists a', In (a', l') ((transfer_presburger_set_binop a l v opc op1 op2)::nil) /\
+               Ensembles.In RegisterMap (gamma a') R'.
+Proof.
+  move => v opc op1 op2 Hop1 Hop2 prog R l R' l' Hstep Hinst a HIn.
+  exists (fst (transfer_presburger_set_binop a l v opc op1 op2)).
+  inversion Hstep. subst.
+  rewrite -Hinst in H6.
+  case: H6 => H6.
+  rewrite H6 /= in H7.
+  split.
+  - left.
+    move: H7 => [HR' Hl'].
+    rewrite Hl'.
+    by reflexivity.
+  - move: (transfer_presburger_set_binop_sound_aux P v opc op1 op2 Hop1 Hop2 R l R' l' H7 a HIn) => Hgoal.
+    by apply Hgoal.
+Qed.
+
 
 Definition transfer_presburger_set {S: Type} {P: PresburgerSet S} (inst: SSA) (s: S) (l: label) :=
-  (top, l+1)::nil.
+  match inst with
+  | Const v c => (transfer_presburger_set_const s l v c)::nil
+  | BinOp v opc op1 op2 op1_ne_v op2_ne_v => (transfer_presburger_set_binop s l v opc op1 op2)::nil
+  end.
+
+Theorem transfer_presburger_set_sound {S: Type} (P: PresburgerSet S) :
+  forall prog R l R' l',
+    step prog (R, l) (R', l') ->
+    forall inst, Some inst = List.nth_error prog l ->
+            forall a, Ensembles.In (total_map Z) (@gamma S (PresburgerSetAD P) a) R ->
+                 exists a', In (a', l') (transfer_presburger_set inst a l) /\
+                       Ensembles.In (total_map Z) (gamma a') R'.
+Proof.
+  move => prog R l R' l' Hstep inst.
+  move: prog R l R' l' Hstep.
+  case inst.
+  - by apply transfer_presburger_set_const_sound.
+  - by apply transfer_presburger_set_binop_sound.
+Qed.
